WIP: proving batch logic

dataplane/Examples/Batch_op_Correctness.thy
@@ -159,9 +159,49 @@ lemma dataflow_tree_to_graph_to_my_summ[simp]:
     done
   done
 
-abbreviation "coll inps t \<equiv> list_of (lmap (\<lambda> e. case e of Data t d \<Rightarrow> d) (lfilter (\<lambda> e. case e of Data t' d \<Rightarrow> t = t' | _ \<Rightarrow> False) inps))"
+definition "coll inps t = list_of (lmap (\<lambda> e. case e of Data t d \<Rightarrow> d) (lfilter (\<lambda> e. case e of Data t' d \<Rightarrow> t = t' | _ \<Rightarrow> False) inps))"
 
-abbreviation "ts inps \<equiv> cimage (\<lambda> e. case e of Data t d \<Rightarrow> t) (cfilter is_Data (cset_of_llist inps))"
+lemma coll_LNil[simp]:
+  "coll LNil t = []"
+  by (auto simp add: coll_def list_of_LCons_conv)
+lemma coll_LCons_Data:
+  "lfinite (lfilter (\<lambda>e. event.time e = t) inps) \<Longrightarrow>
+   coll (LCons (Data t' e) inps) t = (if t = t' then e # coll inps t else coll inps t)"
+   apply (auto simp add: coll_def list_of_LCons_conv)
+  apply (rule FalseE)
+  apply (subgoal_tac "llength (lfilter (\<lambda>e. event.time e = t') inps) \<ge> llength (lfilter (\<lambda>x. case x of Data t'a d \<Rightarrow> t' = t'a | _ \<Rightarrow> False) inps)")
+  subgoal
+    by (metis basic_trans_rules(24) enat_ord_simps(3) llength_eq_infty_conv_lfinite)
+  subgoal premises
+    apply(induct inps)
+    apply (auto intro: order_trans split: event.splits)
+     apply (smt (verit, best) basic_trans_rules(7) eSuc_ile_mono ile_eSuc lfilter_cong)+
+    done
+  done
+lemma coll_LCons_Drop[simp]:
+  "coll (LCons (Drop t') inps) t = coll inps t"
+  by (auto simp add: coll_def list_of_LCons_conv)
+lemma coll_LCons_Mint[simp]:
+  "coll (LCons (Mint t') inps) t = coll inps t"
+  by (auto simp add: coll_def list_of_LCons_conv)
+
+lemma coll_append[simp]:
+  "coll (llist_of (xs @ ys)) t = coll (llist_of xs) t @ coll (llist_of ys) t"
+   apply (simp add: coll_def)
+  done
+
+lemma coll_lshift:
+  "lfinite (lfilter (\<lambda>e. event.time e = t) inps) \<Longrightarrow>
+   coll (xs @@- inps) t = coll (llist_of xs) t @ coll inps t"
+  apply (induct xs arbitrary: inps rule: rev_induct)
+   apply (simp add: coll_def)
+  subgoal for x xs inps
+    apply (cases x)
+   apply (auto simp add: coll_LCons_Data split: event.splits)
+    done
+  done
+
+definition "ts inps = cimage (\<lambda> e. case e of Data t d \<Rightarrow> t) (cfilter is_Data (cset_of_llist inps))"
 
 abbreviation "inp_op os \<equiv> map_op (case_option (Inl (0 :: 2)) (\<lambda> p. Inr (0, p))) (case_option (Inl (0 :: 2)) (\<lambda> p. Inr (0, p))) (ooo_input_op {|1|} os)"
 abbreviation "tt_op os f \<equiv> map_op (case_option (Inl (1 :: 2)) (\<lambda> p. Inr (1, p))) (case_option (Inl (1 :: 2)) (\<lambda> p. Inr (1, p))) (batch_op os f)"
@@ -170,6 +210,95 @@ abbreviation "G_op f ip_state os2 chns \<equiv>
    dataflow_tree_to_operator chns (G f (ip_state :: (1, 'd1 + 'd2, 'd1, _) input_state) (os2 :: (1, 'd1 + 'd2, 'd1, 'd2, _) operator_state_ty2))"
 
 declare if_cong[cong]
+
+definition "cset_from_list = cset_of_llist o llist_of"
+
+lemma cset_from_list_append[simp]:
+  "cset_from_list (xs @ ys) = cUn (cset_from_list xs) (cset_from_list ys)"
+  unfolding cset_from_list_def
+  apply (auto simp flip: cin.rep_eq)
+  done
+lemma cset_from_list_map[simp]:
+  "cset_from_list (map f xs) = (f |`| (cset_from_list xs))"
+  unfolding cset_from_list_def
+  apply (auto simp flip: cin.rep_eq)
+  done
+lemma cset_from_list_concat[simp]:
+  "cset_from_list (concat xs) = cUnion (cset_from_list |`| (cset_from_list xs))"
+  unfolding cset_from_list_def
+  apply (auto simp flip: cin.rep_eq)
+  apply (meson in_cset_of_llist_llist_of rev_cBexI)
+  done
+lemma cset_from_list_rmdups[simp]:
+  "cset_from_list (rmdups {} xs) = cset_from_list xs"
+  unfolding cset_from_list_def
+  apply (auto simp flip: cin.rep_eq)
+  done
+lemma cset_from_list_filter[simp]:
+  "cset_from_list (filter p xs) = cfilter p (cset_from_list xs)"
+  unfolding cset_from_list_def
+  apply (auto simp flip: cin.rep_eq)
+  done
+lemma rcset_cset_from_list[simp]:
+  "rcset (cset_from_list xs) = set xs"
+  unfolding cset_from_list_def
+  apply (auto simp flip: cin.rep_eq)
+  done
+lemma in_cset_from_list[simp]:
+  "x |\<in>| (cset_from_list xs) \<longleftrightarrow> x \<in> set xs"
+  unfolding cset_from_list_def
+  apply (auto simp flip: cin.rep_eq)
+  done
+
+lemma outputs_at_target_my_summ:
+  "outputs_at_target (antichain_from_list oo my_summ) os = (\<lambda> p. if p = (1, 0) then outpu (os 0) 0 else [])"
+  unfolding outputs_at_target_def Src_from_Trg_def my_summ_def
+  apply (rule ext)
+  apply (auto simp add: antichain_from_list_singleton split: prod.splits if_splits)
+  subgoal for nid
+    by (metis Batch_op_Correctness.antichain_from_list_empty Timely_Infrastructure.antichain_from_list_empty)
+  subgoal for nid
+    apply (subgoal_tac "nid = 0")
+     apply simp
+    apply (subgoal_tac "{(nid' :: 2, p' :: 1). antichain_from_list (if nid' = 0 then [0] else []) \<noteq> {}\<^sub>A} = {(0, 1)}")
+    subgoal
+      by (smt (verit, ccfv_SIG) Collect_cong Executable.antichain_from_list_empty antichain_from_list_singleton empty_antichain.abs_eq insert_compr mem_Collect_eq old.prod.case surj_pair
+          the_elem_eq)
+    subgoal premises
+      apply transfer
+      apply auto
+      done
+    done
+  done
+
+lemma coll_llist_of_map_Data[simp]:
+  "coll (llist_of (map (\<lambda>(d, t). Data t (f d)) xs)) t = map (f o fst) (filter (\<lambda> (x, t'). t' = t) xs)"
+  apply (induct xs)
+   apply simp
+  subgoal for x xs
+    apply (cases x)
+    apply (auto simp add: coll_LCons_Data)
+    done
+  done
+
+lemma rcset_ts[simp]:
+  "rcset (ts lxs) = event.time ` {x \<in> (lset lxs). is_Data x}"
+  unfolding ts_def
+  apply (auto simp add:  image_iff cset_of_llist.rep_eq split: event.splits)
+   apply force
+  apply (metis event.distinct(1,3) event.sel(1) is_Data_def)
+  done
+
+lemma snd_cfilter[simp]:
+  "snd |`| cfilter (\<lambda>(d, t). P t) S = cfilter P (snd |`| S)"
+  by (force simp add: image_iff split_beta simp flip: cin.rep_eq)
+
+lemma cset_from_list_image_filter_cfilter:
+  "cset_from_list |`| ((\<lambda>t. map (\<lambda>os. (os, Cap t 1)) (f (map (\<lambda>os. projl (fst os)) (filter (\<lambda>(d, t'). t' = t \<and> P t) xs)))) |`| cfilter P S) =
+   (cset_from_list |`| ((\<lambda>t. map (\<lambda>os. (os, Cap t 1)) (f (map (\<lambda>os. projl (fst os)) (filter (\<lambda>(d, t'). t' = t) xs)))) |`| cfilter P S))"
+  apply auto
+  done
+
 
 lemma correctness_gen:
   fixes inps :: \<open>1 \<Rightarrow> ('t :: {ccompare,canonically_ordered_monoid_add,ordered_ab_semigroup_monoid_add_imp_le,bot}, 'd1) event llist\<close>
@@ -199,12 +328,12 @@ lemma correctness_gen:
     \<open>dataplane_tracker_inv os cbufs sg\<close>
     and S_INV:
     \<open>SP = cUnion (cimage 
-      (\<lambda> t. (cset_of_llist o llist_of) (map (\<lambda> x. ((2, 1), (Inr x, t))) (f (coll ((map (\<lambda> (x, t). Data t (projl x)) (chns (1, 0))) @@- (inps 1)) t))))
-      (cUn (ts (inps 1)) (cset_of_llist (llist_of (map snd (chns (1, 0)))))))\<close>
-    \<open>SO = cset_of_llist (llist_of (map (\<lambda> x. ((2, 1), x)) (outpu (os 1) 0)))\<close>
+      (\<lambda> t. cset_from_list (map (\<lambda> x. ((2, 1), (Inr x, t))) (f (coll ((map (\<lambda> (x, t). Data t (projl x)) (chns (1, 1))) @@- (inps 1)) t))))
+      (cUn (ts (inps 1)) (cset_from_list (map snd (chns (1, 1))))))\<close>
+    \<open>SO = cset_from_list (map (\<lambda> x. ((2, 1), x)) (outpu (os 1) 1))\<close>
     and
     INP_STREAM_INV:
-    \<open>timely_input_stream (inps 0) (mset (ocaps (os 0) 0))\<close>
+    \<open>timely_input_stream (inps 1) (mset (ocaps (os 0) 1))\<close>
   shows 
     \<open>set_op S D (dataflow_op sg (G_op f ip_state bt_state cbufs)) \<approx> set_spec_op (cUn (cUn S SO) SP) D\<close>
   using assms apply -
@@ -284,7 +413,6 @@ proof (coinduction arbitrary: os sg ip_state bt_state chns cbufs inps SP SO S D 
             apply (auto simp add: operator_state.defs comp_def fun_upd_def BTL_def BHD_def Src_from_Trg_def consumes_def add_caps_def BENQ_def my_summ_def BULK_BENQ_def outputs_at_target_def split: option.splits if_splits prod.splits)
             apply (meson UnCI img_fst in_set_tlD)
             done
-          subgoal sorry
           subgoal premises temp
             using SIM1(10) apply -
             apply (rule dataplane_tracker_inv_consumes[where xs="tl (cbufs (1, 1))"])
@@ -301,12 +429,113 @@ proof (coinduction arbitrary: os sg ip_state bt_state chns cbufs inps SP SO S D 
                apply (auto simp add: SIM1 comp_def)
               done
             done
-          subgoal
-            using SIM1(13) by auto
           done
                 defer
         subgoal 
           (* batch_op logic  *)
+   apply (intro exI conjI relcomppI)
+             apply (rule rtranclp.intros(1))
+            apply (rule bisim_refl)
+           defer
+           apply (rule wbisim_refl)
+          apply (rule wb_upto_b_base)
+          unfolding R_def[simplified]
+          apply (rule exI[of _ "os( 1 := (os 1)\<lparr> 
+            outpu := \<lambda>p. outpu (os 1) 1 @
+                   map (\<lambda>x. (Inr (fst x), capability.time (snd x)))
+                    (concat
+                      (map (\<lambda>t. map (\<lambda>x. (x, Cap t 1)) (f (map (\<lambda>x. projl (fst x)) (filter (\<lambda>(d, t'). t' = t \<and> t \<in> set (ocaps (os 1) 1) \<and> \<not> frontier_less_equal (front (os 1) 1) t) (input (os 1) 1)))))
+                        (rmdups {} (map snd (filter (\<lambda>(d, t). t \<in> set (ocaps (os 1) 1) \<and> \<not> frontier_less_equal (front (os 1) 1) t) (input (os 1) 1)))))),
+             ocaps := \<lambda>p. list_diff (ocaps (os 1) 1) (filter (\<lambda>t. \<not> frontier_less_equal (front (os 1) 1) t) (ocaps (os 1) 1)),
+             input := \<lambda>p. filter (\<lambda>(d, t). t \<in> set (ocaps (os 1) 1) \<longrightarrow> frontier_less_equal (front (os 1) 1) t) (input (os 1) 1),
+             produ := produ (os 1) @
+                map (\<lambda>x. (1, capability.time (snd x), 1))
+                 (concat
+                   (map (\<lambda>t. map (\<lambda>x. (x, Cap t 1)) (f (map (\<lambda>x. projl (fst x)) (filter (\<lambda>(d, t'). t' = t \<and> t \<in> set (ocaps (os 1) 1) \<and> \<not> frontier_less_equal (front (os 1) 1) t) (input (os 1) 1)))))
+                     (rmdups {} (map snd (filter (\<lambda>(d, t). t \<in> set (ocaps (os 1) 1) \<and> \<not> frontier_less_equal (front (os 1) 1) t) (input (os 1) 1)))))),
+             inter := operator_state.inter (os 1) @ map (\<lambda>x. (1, x, - 1)) (filter (\<lambda>t. \<not> frontier_less_equal (front (os 1) 1) t) (ocaps (os 1) 1)),
+             nfron := False \<rparr>)"])
+          apply (rule exI[of _ sg])
+          apply (rule exI[of _ "cbufs"])
+          apply (rule exI[of _ inps])
+          apply (rule exI[of _ S])
+          apply (rule exI[of _ D])
+          apply (intro conjI)
+       unfolding dataflow_tree_to_operator_def batch_op_def batch_op_logic_def ooo_input_op_def ooo_input_op_logic_def notifier_op_def
+            apply (simp add: map_tl SIM1(3-) drop_caps_def produces_def comp_def split_beta comp_op_def if_distrib  consumes_def add_caps_def BTL_def enum_num1_def operator_state.defs fun_upd_def)
+              apply (rule arg_cong2[where f=set_spec_op])
+       subgoal premises temp
+       apply (simp add: SIM1(11,12,9))
+         apply (subst (1 2) cUn_assoc)
+               apply (rule arg_cong2[where f=cUn])
+         apply simp
+         apply (simp add: cimage_cUn if_distrib[where f=input] SIM1(1,2) outputs_at_target_my_summ inputs_at_target_def)
+         apply (subst (1) cUn_assoc)
+         apply (rule arg_cong2[where f=cUn])
+         apply simp
+         apply (subst coll_lshift)
+         subgoal sorry
+         apply (subst coll_lshift)
+         subgoal sorry
+         apply (subst coll_lshift)
+         subgoal sorry
+         apply (subst coll_lshift)
+         subgoal sorry
+         unfolding BULK_BENQ_def
+         apply simp
+         apply (simp add: split_beta cimage_cUn)
+         apply (subst (1) cset_from_list_image_filter_cfilter)
+         using cset_from_list_image_filter_cfilter
+
+         find_theorems Set.filter image
+
+end
+           apply (auto 0 0 simp add: image_iff split_beta simp flip: cin.rep_eq)
+           subgoal for t d
+             apply simp_all
+           apply (auto 0 0 simp add: image_iff split_beta simp flip: cin.rep_eq split: event.splits)
+             subgoal for a
+               apply (cases a; simp)
+               subgoal for t' d'
+                 apply hypsubst_thin
+
+
+end
+           apply (auto 0 0 simp add: image_iff split_beta simp flip: cin.rep_eq)
+             apply (subst filter_True)
+             subgoal
+               apply auto
+               subgoal for d' t'
+                 using SIM1(10)[unfolded dataplane_tracker_inv_def, simplified] apply -
+                 apply safe
+                 unfolding front_inv_def imp_front_inv_def
+                 apply (drule spec[of _ 1])
+                 apply (drule spec[of _ 1])
+                 apply (drule spec[of _ "Loc 1 (Trg 1)"])
+                 unfolding chnls_imp_front_inv_def
+                 apply (drule spec[of _ 1])
+                 apply (drule spec[of _ 1])
+                 apply (drule bspec[of _ _ t'])
+                 subgoal
+                   apply (simp add: SIM1(1,2) outputs_at_target_my_summ BULK_BENQ_def)
+
+             thm cimage_eqI
+
+         find_theorems outputs_at_target antichain_from_list
+
+
+end
+         apply (subst (1) cUn_assoc)
+               apply (rule arg_cong2[where f=cUn])
+          apply simp
+         unfolding comp_def
+         apply (simp add: )
+         apply safe
+         subgoal
+
+         find_theorems cset_of_llist llist_of
+
+end
           sorry
         subgoal for st os'
           using SIM1(5) apply simp
